copypasta -> bool flag for gon/hole

Lean/Geo/Hexagon/Encoding.lean
@@ -11,8 +11,8 @@ open LeanSAT Var
 -- a ----------- d
 --   ·         c
 --        b
-def no6Hole3Below (a b c d : Fin n) : PropForm (Var n) :=
-  .not <| .all #[Var.hole a b d, Var.cup a b c, Var.sigma b c d]
+def no6Hole3Below (holes : Bool) (a b c d : Fin n) : PropForm (Var n) :=
+  .not <| .all #[holeIf holes a b d, Var.cup a b c, Var.sigma b c d]
 
 --       .  b
 --   ·         c
@@ -20,7 +20,7 @@ def no6Hole3Below (a b c d : Fin n) : PropForm (Var n) :=
 def no6Hole4Above (a b c d : Fin n) : PropForm (Var n) :=
   .imp (Var.capF a b c) (Var.sigma b c d)
 
-def no6HoleClauses1 (n : Nat) : PropForm (Var n) :=
+def no6HoleClauses1 (n : Nat) (holes : Bool) : PropForm (Var n) :=
   .forAll (Fin n) fun a =>
   .forAll (Fin n) fun b =>
   .guard (a.1+1 < b.1) fun _ =>
@@ -29,16 +29,16 @@ def no6HoleClauses1 (n : Nat) : PropForm (Var n) :=
   .forAll (Fin n) fun d =>
   .guard (c < d) fun _ =>
   .flatCNF <| .all #[
-    no6Hole3Below a b c d,
+    no6Hole3Below holes a b c d,
     .guard (a.1+2 < b.1) fun _ => no6Hole4Above a b c d
   ]
 
 --     ·   p
 -- a --------- c
 --     ·   b
-def no6Hole2Below (a b c p : Fin n) : PropForm (Var n) :=
+def no6Hole2Below (holes : Bool) (a b c p : Fin n) : PropForm (Var n) :=
   .not <| .all #[Var.cup a b c, Var.cap a p c,
-    if b < p then Var.hole a b p else Var.hole a p b]
+    .guard holes fun _ => if b < p then Var.hole a b p else Var.hole a p b]
 
 --        ·
 --   ·         b
@@ -47,7 +47,7 @@ def no6Hole2Below (a b c p : Fin n) : PropForm (Var n) :=
 def no6Hole1Below (a b c p : Fin n) : PropForm (Var n) :=
   .not <| .all #[Var.capF a b c, Var.sigma a p c]
 
-def no6HoleClauses2 (n : Nat) : PropForm (Var n) :=
+def no6HoleClauses2 (n : Nat) (holes : Bool) : PropForm (Var n) :=
   .forAll (Fin n) fun a =>
   .forAll (Fin n) fun b =>
   .guard (a.1 + 1 < b.1) fun _ =>
@@ -56,14 +56,15 @@ def no6HoleClauses2 (n : Nat) : PropForm (Var n) :=
   .forAll (Fin n) fun p =>
   .guard (a < p ∧ p < c ∧ b ≠ p) fun _ =>
   .all #[
-    .guard (a.1 + 1 < p.1) fun _ => no6Hole2Below a b c p,
+    .guard (a.1 + 1 < p.1) fun _ => no6Hole2Below holes a b c p,
     .guard (a.1 + 2 < b.1) fun _ => no6Hole1Below a b c p
   ]
 
-def hexagonEncoding (n : Nat) : PropForm (Var n) :=
-  .all #[baseKGonEncoding n, no6HoleClauses1 n, no6HoleClauses2 n]
+def hexagonEncoding (n : Nat) (holes : Bool) : PropForm (Var n) :=
+  .all #[baseKGonEncoding n holes, no6HoleClauses1 n holes, no6HoleClauses2 n holes]
 
-def hexagonCNF (rlen : Nat) : ICnf := (Geo.hexagonEncoding rlen |>.toICnf compare).2
+def hexagonCNF (rlen : Nat) (holes : Bool) : ICnf :=
+  (Geo.hexagonEncoding rlen holes |>.toICnf compare).2
 
 -- set_option profiler true in
 -- #eval let cnf := Geo.hexagonCNF 30; (cnf.size, cnf.maxVar)
