Lean/Geo/Hexagon/Assn.lean
@@ -11,51 +11,50 @@ namespace Geo.CanonicalPoints
 open List Classical LeanSAT.Model PropFun Point
 attribute [-simp] getElem_fin
 
-theorem satisfies_no6Hole3Below {w : CanonicalPoints} (hw : ¬σHasEmptyKGon 6 w.toFinset)
+theorem satisfies_no6Hole3Below {w : CanonicalPoints} (hw : ¬σHasEmptyKGonIf 6 holes w.toFinset)
     {a c d e : Fin w.rlen} (de : d < e) :
-    (no6Hole3Below a c d e).eval w.toPropAssn := by
+    (no6Hole3Below holes a c d e).eval (w.toPropAssn holes) := by
   simp [no6Hole3Below]; intro ace ⟨b, ab, bc, cd, abc, bcd⟩ cde
-  refine hw <| σCCWPoints.emptyHexagon' ?_ w.gp ace
+  refine hw <| σCCWPoints.emptyHexagonIf' ?_ w.gp ace
     (subset_map w [0, a.succ, b.succ, c.succ, d.succ, e.succ])
   exact Arc.join (l₁ := [_,_,_,_]) (l₂ := [])
     (.cons (Fin.succ_pos _) (w.σ_0 ab) <|
       .cons' ab abc <| .cons' bc bcd <| .cons' cd cde <| .one' de)
     (.one <| Fin.succ_pos _)
 
-theorem satisfies_no6Hole4Above {w : CanonicalPoints} (hw : ¬σHasEmptyKGon 6 w.toFinset)
+theorem satisfies_no6Hole4Above {w : CanonicalPoints} (hw : ¬σHasEmptyKGonIf 6 holes w.toFinset)
     {a d e f : Fin w.rlen} (ef : e < f) :
-    (no6Hole4Above a d e f).eval w.toPropAssn := by
+    (no6Hole4Above a d e f).eval (w.toPropAssn holes) := by
   simp [no6Hole4Above]; intro ⟨de, c, ⟨b, ab, bc, cd, abc, bcd⟩, cde, ace⟩
   refine (w.gp₃' de ef).σ_iff'.1 fun def_ => ?_
-  rw [not_true_eq_false, false_or] at ace
-  refine hw <| (σCCWPoints.cycle (l₂ := [_, _, _, _, _]) ?_).emptyHexagon'
-    w.gp ace.perm₂.perm₁.perm₂ (subset_map' w [f, e, d, c, b, a])
+  refine hw <| (σCCWPoints.cycle (l₂ := [_, _, _, _, _]) ?_).emptyHexagonIf'
+    w.gp (ace · |>.perm₂.perm₁.perm₂) (subset_map' w [f, e, d, c, b, a])
   exact Arc.join (l₁ := []) (l₂ := [_,_,_,_])
     (.one' <| ab.trans <| bc.trans <| cd.trans <| de.trans ef)
     (.cons' ab abc <| .cons' bc bcd <| .cons' cd cde <| .cons' de def_ <| .one' ef)
 
-theorem satisfies_no6Hole2Below {w : CanonicalPoints} (hw : ¬σHasEmptyKGon 6 w.toFinset)
+theorem satisfies_no6Hole2Below {w : CanonicalPoints} (hw : ¬σHasEmptyKGonIf 6 holes w.toFinset)
     {a c e f : Fin w.rlen} :
-    (no6Hole2Below a c f e).eval w.toPropAssn := by
-  simp [no6Hole2Below]; intro ⟨b, ab, bc, cf, abc, bcd⟩ ⟨d, ad, de, ef, ade, def_⟩ hh
+    (no6Hole2Below holes a c f e).eval (w.toPropAssn holes) := by
+  simp [no6Hole2Below]; intro ⟨b, ab, bc, cf, abc, bcd⟩ ⟨d, ad, de, ef, ade, def_⟩
+  refine not_imp.1 fun hh => ?_
   have := Arc.join (l₁ := [_,_]) (l₂ := [_,_])
     (.cons' ab abc <| .cons' bc bcd <| .one' cf)
     (.cons' ad ade <| .cons' de def_ <| .one' ef)
-  refine hw <| this.emptyHexagon w.gp ?_ (subset_map' w [a, b, c, f, e, d])
-  split_ifs at hh with ce <;> simp at hh <;> [exact hh; exact hh.perm₂]
+  refine hw <| this.emptyHexagonIf w.gp (fun h => ?_) (subset_map' w [a, b, c, f, e, d])
+  split_ifs at hh with ce <;> simp [Var.hole] at hh <;> [exact hh h h; exact (hh h h).perm₂]
 
-theorem satisfies_no6Hole1Below {w : CanonicalPoints} (hw : ¬σHasEmptyKGon 6 w.toFinset)
+theorem satisfies_no6Hole1Below {w : CanonicalPoints} (hw : ¬σHasEmptyKGonIf 6 holes w.toFinset)
     {a d e f : Fin w.rlen} (ae : a < e) (ef : e < f) :
-    (no6Hole1Below a d f e).eval w.toPropAssn := by
+    (no6Hole1Below a d f e).eval (w.toPropAssn holes) := by
   simp [no6Hole1Below]; intro ⟨df, c, ⟨b, ab, bc, cd, abc, bcd⟩, cdf, acf⟩ aef
-  rw [not_true_eq_false, false_or] at acf
   have := Arc.join (l₁ := [_]) (l₂ := [_,_,_])
     (.cons' ae aef <| .one' ef)
     (.cons' ab abc <| .cons' bc bcd <| .cons' cd cdf <| .one' df)
-  refine hw <| this.emptyHexagon w.gp acf.perm₂ (subset_map' w [a, e, f, d, c, b])
+  refine hw <| this.emptyHexagonIf w.gp (acf · |>.perm₂) (subset_map' w [a, e, f, d, c, b])
 
-theorem satisfies_hexagonEncoding (w : CanonicalPoints) (hw : ¬σHasEmptyKGon 6 w.toFinset) :
-    (hexagonEncoding w.rlen).eval w.toPropAssn := by with_reducible
+theorem satisfies_hexagonEncoding (w : CanonicalPoints) (hw : ¬σHasEmptyKGonIf 6 holes w.toFinset) :
+    (hexagonEncoding w.rlen holes).eval (w.toPropAssn holes) := by with_reducible
   simp [hexagonEncoding, satisfies_baseKGonEncoding, no6HoleClauses1, no6HoleClauses2]
   refine ⟨
     fun a b _ c _ d cd => ⟨?_, fun _ => ?_⟩,
