Lean/Geo/Hexagon/TheMainTheorem.lean
@@ -5,7 +5,24 @@ import Geo.Hexagon.Encoding
 namespace Geo
 open Classical LeanSAT Model
 
-axiom unsat_6hole_cnf : (Geo.hexagonCNF (rlen := 30-1)).isUnsat
+axiom unsat_6gon_cnf : (Geo.hexagonCNF (rlen := 17-1) (holes := false)).isUnsat
+
+theorem gon_6_theorem (pts : List Point) (gp : Point.ListInGenPos pts)
+    (h : pts.length ≥ 17) : HasConvexKGon 6 pts.toFinset := by
+  refine HasConvexKGon_extension gp (fun pts gp h => ?_) h
+  by_contra h'
+  have noσgon : ¬σHasConvexKGon 6 pts.toFinset := mt (σHasConvexKGon_iff_HasConvexKGon gp).1 h'
+  have ⟨w, ⟨hw⟩⟩ := @symmetry_breaking pts (h ▸ by decide) gp
+  have noσgon' : ¬σHasEmptyKGonIf 6 (holes := false) w.toFinset :=
+    OrientationProperty_σHasConvexKGon.not (hw.toEquiv w.nodup) noσgon
+  have rlen_eq : w.rlen = 16 := Nat.succ_inj.1 <| hw.length_eq.symm.trans h
+  apply unsat_6gon_cnf
+  with_reducible
+    have := (PropForm.toICnf_sat _).2 ⟨w.toPropAssn false, w.satisfies_hexagonEncoding noσgon'⟩
+    rw [rlen_eq] at this
+    rwa [hexagonCNF]
+
+axiom unsat_6hole_cnf : (Geo.hexagonCNF (rlen := 30-1) (holes := true)).isUnsat
 
 theorem hole_6_theorem (pts : List Point) (gp : Point.ListInGenPos pts)
     (h : pts.length ≥ 30) : HasEmptyKGon 6 pts.toFinset := by
@@ -13,7 +30,7 @@ theorem hole_6_theorem (pts : List Point) (gp : Point.ListInGenPos pts)
   by_contra h'
   have noσtri : ¬σHasEmptyKGon 6 pts.toFinset := mt (σHasEmptyKGon_iff_HasEmptyKGon gp).1 h'
   have ⟨w, ⟨hw⟩⟩ := @symmetry_breaking pts (h ▸ by decide) gp
-  have noσtri' : ¬σHasEmptyKGon 6 w.toFinset :=
+  have noσtri' : ¬σHasEmptyKGonIf 6 (holes := true) w.toFinset :=
     OrientationProperty_σHasEmptyKGon.not (hw.toEquiv w.nodup) noσtri
   have rlen29 : w.rlen = 29 := Nat.succ_inj.1 <| hw.length_eq.symm.trans h
   apply unsat_6hole_cnf
@@ -21,6 +38,12 @@ theorem hole_6_theorem (pts : List Point) (gp : Point.ListInGenPos pts)
     have := (PropForm.toICnf_sat _).2 ⟨w.toPropAssn, w.satisfies_hexagonEncoding noσtri'⟩
     rw [rlen29] at this
     rwa [hexagonCNF]
+
+/--
+info: 'Geo.gon_6_theorem' depends on axioms:
+[propext, Classical.choice, Quot.sound, Geo.unsat_6gon_cnf, mathlibSorry]
+-/
+#guard_msgs in #print axioms gon_6_theorem
 
 /--
 info: 'Geo.hole_6_theorem' depends on axioms:
